coq/LLVMGen/Vellvm_Utils.v
@@ -22,7 +22,8 @@ From Vellvm Require Import
      Handlers.Handlers
      Theory.Refinement
      Theory.DenotationTheory
-     Theory.InterpreterCFG.
+     Theory.InterpreterCFG
+     Theory.InterpreterMCFG.
 
 From ExtLib Require Import
      Structures.Functor.
@@ -32,7 +33,9 @@ From Coq Require Import
      Logic
      Morphisms
      Relations
-     List.
+     List
+     Program
+     ZArith.
 
 Require Import Ceres.Ceres.
 Import BinInt.
@@ -90,20 +93,23 @@ Module eutt_Notations.
          ).
 End eutt_Notations.
 
-Import D. 
+Import D.
 Module VIR_denotation_Notations.
   (* Notation "'ℐ' '(' t ')' g l m" := (interp_cfg_to_L3 _ t g l m) (only printing, at level 10). *)
   Notation "'global.' g 'local.' l 'memory.' m 'ℐ' t" :=
     (interp_cfg3 t g l m)
       (only printing, at level 10,
        format "'global.'  g '//' 'local.'  l '//' 'memory.'  m '//' 'ℐ'  t").
-  
+
   Notation "⟦ c ⟧" := (denote_code c) (only printing, at level 10).
   Notation "⟦ i ⟧" := (denote_instr i) (only printing, at level 10).
   Notation "⟦ t ⟧" := (denote_terminator t) (only printing, at level 10).
   Notation "⟦ e ⟧" := (denote_exp None e) (only printing, at level 10).
   Notation "⟦ τ e ⟧" := (denote_exp (Some τ) e) (only printing, at level 10).
   Notation "x" := (translate exp_to_instr x) (only printing, at level 10).
+
+  (* Should be part of the surface notations *)
+  Notation "'call' x args" := ((IVoid _, INSTR_Call x args)) (at level 30, only printing).
 
   Notation "'λ' a b c d ',' k" := (fun '(a,(b,(c,d))) => k) (only printing, at level 0, format "'λ'  a  b  c  d ',' '[' '//' k ']'").
 
@@ -151,4 +157,763 @@ From Vellvm Require Import
 .
 Require Export ITree.Events.FailFacts.
 
+From Vellvm Require Import Utils.PostConditions.
+
+(** * Naming conventions for configurations and predicates over configurations *)
+
+Notation memoryV := memory_stack.
+
+(* Return state of a denoted and interpreted [cfg].
+     Note the lack of local stack *)
+Definition config_cfg
+  := memoryV * (local_env * (global_env)).
+
+(* Constructor to avoid having to worry about the nesting *)
+Definition mk_config_cfg m l g: config_cfg := (m,(l,g)).
+
+(* Return state of a denoted and interpreted [mcfg] *)
+Definition config_mcfg
+  := memoryV *
+       (local_env * @Stack.stack (local_env) * (global_env)).
+
+(* Return state and value of a denoted and interpreted (open) [cfg].
+     Note the lack of local stack.
+     Note that we may return a [block_id] alternatively to a [uvalue]
+ *)
+Definition config_cfg_T (T:Type): Type
+  := memoryV * (local_env * (global_env * T)).
+Definition config_res_cfg
+  := config_cfg_T (block_id + uvalue).
+
+(* Return state and value of a denoted and interpreted [mcfg]. *)
+Definition config_mcfg_T (T:Type): Type
+  := memoryV * (local_env * @Stack.stack (local_env) * (global_env * T)).
+Definition config_res_mcfg :=
+  config_mcfg_T uvalue.
+
+(* -- Injections -- *)
+(* The nested state transformers associate the products the other way,
+     we therefore define injections of memory states and values into return
+     types of computations.
+ *)
+Definition mk_config_cfg_T (T:Type) (v:T): config_cfg -> (config_cfg_T T)
+  := fun '(m, (ρ, g)) => (m, (ρ, (g, v))).
+
+Definition mk_config_mcfg_T (T:Type) (v:T): config_mcfg -> (config_mcfg_T T)
+  := fun '(m, (ρ, g)) => (m, (ρ, (g, v))).
+
+
+(* Facilities to refer to the type of relations used during the simulations
+   of various pieces of denotions we manipulate.
+   In particular, all relations we state assume success on the Helix side, and
+   we will lift systematically these relations to the option type.
+ *)
+
+(** * Predicates  *)
+(** Predicate on mcfg-level states *)
+Definition Pred_mcfg: Type := config_mcfg -> Prop.
+Definition Pred_mcfg_T (TV: Type): Type := config_mcfg_T TV -> Prop.
+(** Predicate on cfg-level states *)
+Definition Pred_cfg: Type := config_cfg -> Prop.
+Definition Pred_cfg_T (TV: Type): Type := config_cfg_T TV -> Prop.
+
+Require Import ExtLib.Data.Map.FMapAList.
+Import SemNotations.
+
+(** * Specifications for alloc *)
+
+Lemma allocated_allocate_allocated (m1 m2 : memoryV) (d : dtyp) (a a' : Addr.addr) :
+  allocated a m1 -> allocate m1 d = inr (m2, a') -> allocated a m2.
+Proof.
+  intros A AS.
+  unfold allocate, allocated in *.
+  destruct d; inv AS.
+  all: repeat break_let; subst.
+  all: unfold add_logical_block, add_logical_block_mem, add_to_frame in *.
+  all: repeat break_match; inv Heqm1.
+  all: apply member_add_ineq; [| assumption].
+  all: unfold next_logical_key, next_logical_key_mem.
+  all: simpl.
+  all: intros C; rewrite C in A; contradict A.
+  all: apply next_logical_key_fresh.
+Qed.
+
+Lemma allocate_allocated (m1 m2 : memoryV) (d : dtyp) (a : Addr.addr) :
+  allocate m1 d = inr (m2, a) -> allocated a m2.
+Proof.
+  intros AS.
+  unfold allocate, allocated in *.
+  destruct d; inv AS.
+  all: repeat break_let; subst.
+  all: unfold add_logical_block, add_logical_block_mem, add_to_frame in *.
+  all: repeat break_match; inv Heqm; inv Heqm0.
+  all: apply member_add_eq.
+Qed.
+
+(** * MISC *)
+
+Lemma eutt_trans : forall {E A} (R : A -> A -> Prop),
+    Transitive R ->
+    Transitive (eutt (E := E) R).
+Proof.
+  repeat intro.
+  eapply eqit_trans in H1; [| apply H0].
+  eapply eqit_mon with (RR := rcompose R R); eauto.
+  intros.
+  apply trans_rcompose; eauto.
+Qed.
+
+Lemma eutt_ret_inv_strong {E X Y} (R : X -> Y -> Prop) (x : X) (t : itree E Y) :
+  eutt R (Ret x) t ->
+  exists y, t ≈ Ret y /\ R x y.
+Proof.
+  intros EQ; punfold EQ.
+  red in EQ.
+  dependent induction EQ.
+  - exists r2; split; auto.
+    rewrite itree_eta, <-x; reflexivity.
+  - edestruct IHEQ as (y & EQ1 & HR); auto.
+    exists y; split; auto.
+    now rewrite itree_eta, <- x, tau_eutt.
+Qed.
+
+Lemma eutt_ret_inv_strong' {E X Y} (R : X -> Y -> Prop) (t : itree E X) (y : Y) :
+  eutt R t (Ret y) ->
+  exists x, t ≈ Ret x /\ R x y.
+Proof.
+  intros EQ; punfold EQ.
+  red in EQ.
+  dependent induction EQ.
+  - exists r1; split; auto.
+    rewrite itree_eta, <-x; reflexivity.
+  - edestruct IHEQ as (?x & EQ1 & HR); auto.
+    exists x0; split; auto.
+    now rewrite itree_eta, <- x, tau_eutt.
+Qed.
+
+Lemma typ_to_dtyp_void s : typ_to_dtyp s TYPE_Void = DTYPE_Void.
+Proof.
+  intros; rewrite typ_to_dtyp_equation; reflexivity.
+Qed.
+
+Lemma option_rel_trans : forall {A} (R : A -> A -> Prop),
+    Transitive R ->
+    Transitive (option_rel R).
+Proof.
+  repeat intro.
+  cbv in *.
+  repeat break_match; intuition.
+  subst.
+  eapply H; eauto.
+Qed.
+
+Lemma exp_eq_dec: forall e1 e2 : exp dtyp, {e1 = e2} + {e1 <> e2}.
+Admitted.
+
+Lemma global_eq_dec: forall g1 g2 : global dtyp, {g1 = g2} + {g1 <> g2}.
+Proof.
+  repeat decide equality.
+  apply exp_eq_dec.
+  apply dtyp_eq_dec.
+Qed.
+
+(** * [interp_local_stack] theory *)
+Lemma interp_local_stack_tau:
+  forall (k v map : Type) (M : Maps.Map k v map) (SK : CeresSerialize.Serialize k) (E F G : Type -> Type) (H : FailureE -< E +' F +' G) (R : Type) (l : map * stack) (t : itree (E +' F +' (LocalE k v +' StackE k v) +' G) R),
+    interp_local_stack (Tau t) l ≅ Tau (interp_local_stack t l).
+Proof.
+  intros.
+  unfold interp_local_stack at 1.
+  rewrite interp_state_tau.
+  reflexivity.
+Qed.
+
+
+(** * [interp_mcfg3] theory *)
+
+Lemma interp3_ret : forall (R : Type) (g : global_env) (l : local_env * stack) (m : memoryV) (x : R), ℑs3 (Ret x) g l m ≅ Ret3 g l m x.
+Proof.
+  intros; unfold ℑs3.
+  rewrite interp_intrinsics_ret, interp_global_ret, interp_local_stack_ret, interp_memory_ret.
+  reflexivity.
+Qed.
+
+Lemma interp3_tau : forall R (t : itree L0 R) g l m,
+    interp_mcfg3 (Tau t) g l m ≅ Tau (interp_mcfg3 t g l m).
+Proof.
+  intros; unfold ℑs3.
+  rewrite interp_intrinsics_Tau, interp_global_Tau, interp_local_stack_tau, interp_memory_Tau.
+  reflexivity.
+Qed.
+
+Lemma interp3_map_monad {A B} g l m (xs : list A) (ts : A -> itree _ B) :
+  ℑs3 (map_monad ts xs) g l m ≈
+    map_monad (m := Monads.stateT _ (Monads.stateT _ (Monads.stateT _ (itree _))))
+    (fun a => ℑs3 (ts a)) xs g l m.
+Proof.
+  intros; revert g l m; induction xs as [| a xs IH]; simpl; intros.
+  - rewrite interp3_ret; reflexivity.
+  - rewrite interp3_bind.
+    apply eutt_eq_bind; intros (? & ? & ? & ?); cbn.
+    rewrite interp3_bind, IH.
+    apply eutt_eq_bind; intros (? & ? & ? & ?); cbn.
+    rewrite interp3_ret; reflexivity.
+Qed.
+
+Instance eq_itree_interp3:
+  forall T : Type, Proper (eq_itree eq ==> eq ==> eq ==> eq ==> eq_itree eq) (@interp_mcfg3 T).
+Proof.
+  repeat intro.
+  unfold ℑs3.
+  subst; rewrite H.
+  reflexivity.
+Qed.
+
+Lemma interp3_MemPush: forall g l m,
+    ℑs3 (trigger MemPush) g l m ≈ Ret3 g l (push_fresh_frame m) tt.
+Proof.
+  intros.
+  unfold ℑs3.
+  MCFGTactics.go.
+  rewrite interp_memory_trigger.
+  cbn.
+  MCFGTactics.go.
+  reflexivity.
+Qed.
+
+Lemma interp3_StackPush: forall g a sbot m s,
+    ℑs3 (trigger (StackPush s)) g (a,sbot) m ≈
+      Ret3 g (fold_right (fun '(x, dv) => alist_add x dv) [] s, a :: sbot) m tt.
+Proof.
+  intros.
+  unfold ℑs3.
+  MCFGTactics.go.
+  reflexivity.
+Qed.
+
+Lemma interp3_GR : forall id g l m v,
+  Maps.lookup id g = Some v ->
+  interp_mcfg3 (trigger (GlobalRead id)) g l m ≈ Ret (m,(l,(g,v))).
+Proof.
+  intros * LU.
+  unfold interp_mcfg3.
+  rewrite interp_intrinsics_trigger.
+  cbn.
+  unfold Intrinsics.F_trigger.
+  rewrite interp_global_trigger.
+  cbn in *; rewrite LU.
+  rewrite interp_local_stack_ret, interp_memory_ret.
+  reflexivity.
+Qed.
+
+Lemma interp3_denote_exp_double : forall t g l m,
+    interp_mcfg3
+      (translate exp_to_L0
+                 (denote_exp (Some (DTYPE_Double))
+                             (EXP_Double t)))
+      g l m
+    ≈
+    Ret (m, (l, (g, UVALUE_Double t))).
+Proof.
+  intros; unfold denote_exp; cbn.
+  rewrite translate_ret, interp3_ret.
+  reflexivity.
+Qed.
+
+Lemma interp3_denote_exp_i64 : forall t g l m,
+    interp_mcfg3
+      (translate exp_to_L0
+                 (denote_exp (Some (DTYPE_I 64))
+                             (EXP_Integer (unsigned t))))
+       g l m
+    ≈
+    Ret (m, (l, (g, UVALUE_I64 (DynamicValues.Int64.repr (unsigned t))))).
+Proof.
+  intros; unfold denote_exp; cbn.
+  rewrite translate_ret, interp3_ret.
+  reflexivity.
+Qed.
+
+Lemma interp3_concretize_or_pick_concrete :
+  forall (uv : uvalue) (dv : dvalue) P g ρ m,
+    is_concrete uv ->
+    uvalue_to_dvalue uv = inr dv ->
+    interp_mcfg3 (concretize_or_pick uv P) g ρ m ≈ Ret (m, (ρ, (g, dv))).
+Proof.
+  intros uv dv P g ρ m CONC CONV.
+  unfold concretize_or_pick.
+  rewrite CONC.
+  cbn.
+  unfold lift_err.
+  now rewrite CONV, interp3_ret.
+Qed.
+
+Lemma interp3_concretize_or_pick_concrete_exists :
+  forall (uv : uvalue) P g ρ m,
+    is_concrete uv ->
+    exists dv, uvalue_to_dvalue uv = inr dv /\
+          interp_mcfg3 (concretize_or_pick uv P) g ρ m ≈ Ret (m, (ρ, (g, dv))).
+Proof.
+  intros uv P g ρ m CONC.
+  pose proof is_concrete_uvalue_to_dvalue uv CONC as (dv & CONV).
+  exists dv.
+  split; auto.
+  now apply interp3_concretize_or_pick_concrete.
+Qed.
+
+Lemma interp3_store:
+  forall (m m' : memoryV) (val : dvalue) (a : addr) g l,
+    write m a val = inr m' ->
+    interp_mcfg3 (trigger (Store (DVALUE_Addr a) val)) g l m ≈ Ret (m', (l, (g, ()))).
+Proof.
+  intros m m' val a g l WRITE.
+  unfold interp_mcfg3.
+  rewrite interp_intrinsics_trigger.
+  cbn.
+  unfold Intrinsics.F_trigger.
+  rewrite interp_global_trigger.
+  rewrite subevent_subevent.
+  cbn.
+  rewrite interp_local_stack_bind, interp_local_stack_trigger.
+  cbn; rewrite subevent_subevent.
+  rewrite Eq.bind_bind.
+  rewrite interp_memory_bind, interp_memory_store; eauto.
+  cbn; rewrite Eq.bind_ret_l.
+  rewrite interp_memory_bind, interp_memory_ret, Eq.bind_ret_l.
+  rewrite interp_local_stack_ret, interp_memory_ret.
+  reflexivity.
+Qed.
+
+(** * [interp_mrec] theory *)
+
+#[local] Definition mcfg_ctx fundefs :
+  forall T : Type,
+    CallE T
+    -> itree (CallE +' ExternalCallE +' IntrinsicE +' LLVMGEnvE +' (LLVMEnvE +' LLVMStackE) +' MemoryE +' PickE +' UBE +' DebugE +' FailureE) T :=
+
+  (fun (T : Type) (call : CallE T) =>
+    match call in (CallE T0) return (itree (CallE +' ExternalCallE +' IntrinsicE +' LLVMGEnvE +' (LLVMEnvE +' LLVMStackE) +' MemoryE +' PickE +' UBE +' DebugE +' FailureE) T0) with
+    | LLVMEvents.Call dt0 fv args0 =>
+        dfv <- concretize_or_pick fv True;;
+        match lookup_defn dfv fundefs with
+        | Some f_den => f_den args0
+        | None =>
+            dargs <- map_monad (fun uv : uvalue => pickUnique uv) args0;;
+            Functor.fmap dvalue_to_uvalue (trigger (ExternalCall dt0 fv dargs))
+        end
+    end).
+
+Lemma denote_mcfg_unfold_in : forall G τ addr args f,
+    lookup_defn (DVALUE_Addr addr) G = Some f ->
+    denote_mcfg G τ (UVALUE_Addr addr) args ≈
+      interp_mrec (mcfg_ctx G) (f args).
+Proof.
+  intros * LU.
+  unfold denote_mcfg at 1.
+  rewrite RecursionFacts.mrec_as_interp.
+  simpl bind. rewrite interp_bind.
+  cbn.
+  rewrite interp_ret, bind_ret_l.
+  rewrite LU.
+  rewrite <- RecursionFacts.interp_mrec_as_interp.
+  reflexivity.
+Qed.
+
+Lemma interp_mrec_ret :
+  forall (D E : Type -> Type) (ctx : forall T : Type, D T -> itree (D +' E) T) (U : Type) (u : U),
+    interp_mrec ctx (Ret u) ≅ (Ret u).
+Proof.
+  intros.
+  rewrite unfold_interp_mrec; reflexivity.
+Qed.
+
+Lemma interp_mrec_tau : forall D E (ctx : D ~> itree (D +' E)) R (t : itree _ R),
+    interp_mrec ctx (Tau t) ≅ Tau (interp_mrec ctx t).
+Proof.
+  intros.
+  now rewrite unfold_interp_mrec.
+Qed.
+
+#[global] Instance interp_mrec_eutt {D E}
+  (ctx : D ~> itree (D +' E)) T :
+  Proper (eutt eq ==> eutt eq) (interp_mrec ctx (T := T)).
+Proof.
+  repeat intro.
+  eapply Proper_interp_mrec; auto.
+  intros ??.
+  reflexivity.
+Qed.
+
+Lemma interp3_call_void : forall G n τ f fdfn args g s m addr,
+    prefix "llvm." f = false ->
+    Maps.lookup (Name f) g = Some (DVALUE_Addr addr) ->
+    lookup_defn (DVALUE_Addr addr) G = Some fdfn ->
+
+    ℑs3 (interp_mrec (mcfg_ctx G)
+           (Interp.translate instr_to_L0'
+              ⟦(IVoid n, INSTR_Call (τ, EXP_Ident (ID_Global (Name f))) args) ⟧i)) g s m
+      ≈
+      '(m,(s,(g,vs))) <- ℑs3 (interp_mrec (mcfg_ctx G)
+                               (Interp.translate instr_to_L0'
+                                  (map_monad (fun '(t, op) => Interp.translate exp_to_instr ⟦ op at t ⟧e) args))) g s m
+    ;;
+
+    '(m,(s,(g,v))) <- ℑs3 (interp_mrec (mcfg_ctx G) (fdfn vs)) g s m;;
+    Ret (m,(s,(g,tt))).
+Proof.
+  intros * PRE LU LUD.
+  Transparent denote_instr.
+  cbn.
+  rewrite translate_bind, interp_mrec_bind, interp3_bind.
+  (* Expressions are pure, lifted by induction over map_monad *)
+  apply eutt_clo_bind with
+    (UU := fun '(m1,(s1,(g1,v))) m2 =>
+             (m1,(s1,(g1,v))) = m2 /\ m1 = m /\ s1 = s /\ g1 = g).
+  admit.
+  intros (m1,(s1,(g1,v1))) (m2,(s2,(g2,v2))) (EQ & -> & -> & ->).
+  symmetry in EQ; inv EQ.
+  rewrite PRE.
+  (* repeat break_and. *)
+  rewrite bind_bind.
+  rewrite translate_bind, interp_mrec_bind, interp3_bind.
+  Transparent denote_exp.
+  unfold denote_exp.
+  cbn.
+  rewrite bind_trigger.
+  rewrite translate_vis.
+  rewrite translate_vis.
+  rewrite translate_vis.
+  cbn.
+  rewrite <- bind_trigger.
+  rewrite interp_mrec_bind.
+  rewrite interp_mrec_trigger.
+  cbn.
+  rewrite interp3_bind.
+  match goal with
+    |- context[ℑs3 ?e] =>
+      let eqn := fresh in
+      assert (eqn:e = trigger (@GlobalRead raw_id dvalue (Name f))) by reflexivity;
+      rewrite eqn; clear eqn
+  end.
+  rewrite interp3_GR; [| apply LU].
+  rewrite bind_ret_l.
+  rewrite 3translate_ret.
+  rewrite interp_mrec_ret, interp3_ret, bind_ret_l.
+
+  rewrite !translate_bind, interp_mrec_bind, interp3_bind.
+  rewrite translate_trigger, interp_mrec_trigger.
+  cbn.
+  rewrite mrec_as_interp.
+  cbn.
+  rewrite bind_ret_l.
+  rewrite LUD.
+  cbn.
+  rewrite <- RecursionFacts.interp_mrec_as_interp.
+
+  apply eutt_eq_bind.
+  intros (? & ? & ? & ?).
+  rewrite translate_ret, interp_mrec_ret, interp3_ret.
+  reflexivity.
+  Opaque denote_instr.
+  Opaque denote_exp.
+
+Admitted.
+
+(* Weirdly specific... Shouldn't we lift results that do not depend on [interp_mrec]? *)
+Lemma denote_mcfg_ID_Global :
+  forall ctx (g : global_env) s (m : memoryV) id (τ : dtyp) (ptr : Addr.addr),
+    alist_find id g = Some (DVALUE_Addr ptr) ->
+
+    ℑs3 (interp_mrec ctx
+           (Interp.translate instr_to_L0'
+              (Interp.translate exp_to_instr (denote_exp (Some τ) (EXP_Ident (ID_Global id)))))) g s m
+      ≈
+      Ret3 g s m (UVALUE_Addr ptr)
+.
+Proof.
+  intros * LU.
+  Transparent denote_exp.
+  unfold denote_exp.
+  cbn.
+  rewrite 3translate_bind, interp_mrec_bind, interp3_bind.
+  rewrite !translate_trigger.
+  cbn.
+  rewrite interp_mrec_trigger.
+  cbn.
+
+  match goal with
+    |- context[ℑs3 ?e] =>
+      let eqn := fresh in
+      assert (eqn:e = trigger (@GlobalRead raw_id dvalue id)) by reflexivity;
+      rewrite eqn; clear eqn
+  end.
+
+  rewrite interp3_GR; [| apply LU].
+  rewrite bind_ret_l.
+  rewrite !translate_ret,interp_mrec_ret,interp3_ret.
+  reflexivity.
+Qed.
+
+(** * [allocate_globals] theory *)
+
+Import AlistNotations.
+Definition global_ptr_exists fnname : Pred_mcfg :=
+  fun '(mem_llvm, (ρ,g)) => exists mf, g @ fnname = Some (DVALUE_Addr mf).
+
+Definition global_ptr_existsT {T} fnname : Pred_mcfg_T T :=
+  fun '(mem_llvm, (ρ,(g,_))) => exists mf, g @ fnname = Some (DVALUE_Addr mf).
+
+Record gs_wf (gs : list (global dtyp)) : Prop :=
+  {
+    gs_wf_nodup  : NoDup (List.map g_ident gs);
+    gs_wf_novoid : Forall (fun x => non_void (g_typ x)) gs
+  }.
+
+Definition global_is_init (g : global_env) (m : memoryV) (glob : global dtyp) : Prop :=
+  exists mf, g @ (g_ident glob) = Some (DVALUE_Addr mf) /\ allocated mf m.
+
+Definition globals_are_uniquely_init (g : global_env) (globs : list (global dtyp)) : Prop :=
+  forall glob glob', In glob globs -> In glob' globs -> g_ident glob <> g_ident glob' ->
+                g @ (g_ident glob) <> g @ (g_ident glob').
+
+(* TODO
+   [gs_init_fresh] should be replaced by a predicate specifying
+   the current domain of [g], and take into account the declarations
+   that have already be allocated
+ *)
+Record init_globals (globs : list (global dtyp)) (g : global_env) (m : memoryV) : Prop :=
+  {
+    gs_init          : Forall (global_is_init g m) globs;
+    gs_init_distinct : globals_are_uniquely_init g globs;
+    gs_init_fresh    : forall id, ~ In id (map g_ident globs) -> g @ id = None
+  }
+.
+
+Definition init_globalsT {T} globs : Pred_mcfg_T T :=
+  fun '(m, (_,(g,_))) => init_globals globs g m.
+
+(*   In (dc_name d) (map dc_name IntrinsicsDefinitions.defined_intrinsics_decls) *)
+(*   \/  *)
+(* . *)
+
+(* exists mf, g @ (g_ident glob) = Some (DVALUE_Addr mf) *)
+(*         /\ allocated mf m. *)
+
+
+(* Record init_decls (decls : list (declaration dtyp)) *)
+(*   (g : global_env) (m : memoryV) : Prop := *)
+(*   { *)
+(*     gs_init_decls          : Forall (global_is_init g m) globs; *)
+(*     gs_init_distinct_decls : globals_are_uniquely_init g globs; *)
+(*     gs_init_fresh_decls    : forall id, ~ In id (map g_ident globs) -> g @ id = None *)
+(*   } *)
+(* . *)
+
+
+(* Lemma allocate_declaration_spec : forall (d : declaration dtyp), *)
+(*     allocate_declaration d ⤳  *)
+
+
+(* One proper round of global initialization preserves the invariant *)
+Lemma gs_init_extend :
+  forall g m m' τ a (glob : global dtyp) globs v,
+    ~ In (g_ident glob) (map g_ident globs) ->
+    init_globals globs g m ->
+    allocate m τ = inr (m', a) ->
+    Forall (global_is_init (alist_add (g_ident glob) v g) m') globs.
+Proof.
+  intros * NIN [FA _ FR] AS.
+  rewrite Forall_forall in FA.
+  apply Forall_forall.
+  intros * IN; apply FA in IN as (? & EQ & AL).
+  eexists.
+  split.
+  - rewrite alist_find_neq.
+    apply EQ.
+    intros abs.
+    apply FR in NIN.
+    rewrite <- abs, EQ in NIN.
+    inv NIN.
+  - eapply allocated_allocate_allocated; eauto.
+Qed.
+
+Lemma allocate_global_spec : forall (glob : global dtyp) globs g s m,
+    non_void (g_typ glob) ->
+    ~ In (g_ident glob) (map g_ident globs) ->
+    init_globals globs g m ->
+    ℑs3 (allocate_global glob) g s m ⤳ init_globalsT (glob :: globs).
+Proof.
+  intros * NV FR INV; pose proof INV as [].
+  unfold allocate_global.
+  cbn.
+  rewrite interp3_bind.
+  edestruct interp3_alloca as (? & mf & ? & EQ); [eauto |].
+  rewrite EQ; clear EQ.
+  cbn; rewrite bind_ret_l.
+  rewrite interp3_GW.
+  apply eutt_Ret.
+  cbn.
+  split.
+  - apply Forall_cons; auto.
+    2: eapply gs_init_extend; eauto.
+    eexists.
+    split.
+    rewrite alist_find_add_eq; reflexivity.
+    eapply allocate_allocated; eauto.
+  - intros ? ? IN IN' NEQ.
+    destruct IN as [<- | IN].
+    + rewrite alist_find_add_eq.
+      destruct IN' as [<- | IN'].
+      * now contradiction NEQ.
+      * rewrite alist_find_neq; auto.
+        eapply Forall_forall in gs_init0; [| apply IN'].
+        destruct gs_init0 as (mf' & EQ & AL).
+        unfold global_id in *; rewrite EQ.
+        intros abs; inv abs.
+        apply allocate_correct, was_fresh in H.
+        intuition.
+    + destruct IN' as [<- | IN'].
+      * rewrite alist_find_neq; auto.
+        rewrite alist_find_add_eq.
+        eapply Forall_forall in gs_init0; [| apply IN].
+        destruct gs_init0 as (mf' & EQ & AL).
+        unfold global_id in *; rewrite EQ.
+        intros abs; inv abs.
+        apply allocate_correct, was_fresh in H.
+        intuition.
+      * rewrite 2 alist_find_neq; auto.
+        all:intros abs; apply FR; rewrite <- abs; now apply in_map.
+  - intros * NIN.
+    destruct (raw_id_eq_dec id (g_ident glob)).
+    + subst.
+      exfalso; apply NIN; left; reflexivity.
+    + rewrite alist_find_neq; auto.
+      apply gs_init_fresh0.
+      intros abs; apply NIN; right; auto.
+Qed.
+
+
+Lemma allocate_globals_cons :
+  forall g gs,
+    allocate_globals (g :: gs) ≈ allocate_global g;; allocate_globals gs.
+Proof.
+  intros; cbn.
+  rewrite !bind_bind.
+  apply eutt_eq_bind; intros ?.
+  apply eutt_eq_bind; intros ?.
+  rewrite !bind_bind.
+  apply eutt_eq_bind; intros ?.
+  rewrite bind_ret_l.
+  reflexivity.
+Qed.
+
+Lemma init_globals_shuffle_snoc : forall glob globs g m,
+      init_globals  (glob :: globs) g m ->
+      init_globals (globs ++ [glob]) g m.
+Proof.
+  intros * [].
+  constructor.
+  - apply Forall_app; apply List.Forall_cons_iff in gs_init0 as [? ?].
+    split; auto.
+  - intros ? ? IN IN' NEQ.
+    apply in_app_or in IN, IN'.
+    apply gs_init_distinct0; auto.
+    destruct IN as [IN | IN]; [right; auto| destruct IN as [<- |[]]; left; reflexivity].
+    destruct IN' as [IN' | IN']; [right; auto| destruct IN' as [<- |[]]; left; reflexivity].
+  - intros ? NIN.
+    apply gs_init_fresh0; auto.
+    intros abs; apply NIN; destruct abs as [<- | IN].
+    rewrite map_app; apply in_or_app; right; left; reflexivity.
+    rewrite map_app; apply in_or_app; now left.
+Qed.
+
+Lemma init_globalsT_shuffle_snoc : forall {T} glob globs cfn,
+      init_globalsT (T := T) (glob :: globs) cfn ->
+      init_globalsT (globs ++ [glob]) cfn.
+Proof.
+  intros ??? [m' [ρ' [g' ?]]]. apply init_globals_shuffle_snoc.
+Qed.
+
+Lemma init_globals_shuffle_snoc' : forall glob globs g m,
+      init_globals (globs ++ [glob]) g m ->
+      init_globals (glob :: globs) g m.
+Proof.
+  intros * [].
+  constructor.
+  - apply Forall_app in gs_init0 as [? ?]; apply List.Forall_cons_iff.
+    inv H0; split; auto.
+  - intros ? ? IN IN' NEQ.
+    apply gs_init_distinct0; auto.
+    apply in_or_app; destruct IN as [<- | IN]; auto; right; left; auto.
+    apply in_or_app; destruct IN' as [<- | IN']; auto; right; left; auto.
+  - intros ? NIN.
+    apply gs_init_fresh0; auto.
+    intros abs; apply NIN. rewrite map_app in abs.
+    apply in_app_or in abs.
+    cbn.
+    destruct abs; auto.
+    destruct H; auto.
+    contradiction H.
+Qed.
+
+Lemma init_globalsT_shuffle_snoc' : forall {T} glob globs cfn,
+      init_globalsT (globs ++ [glob]) cfn ->
+      init_globalsT (T := T) (glob :: globs) cfn.
+Proof.
+  intros ??? [m' [ρ' [g' ?]]]. apply init_globals_shuffle_snoc'.
+Qed.
+
+Lemma allocate_globals_spec_gen :
+  forall (globs_todo globs_done : list (global dtyp)) (g : global_env) s m,
+    NoDup (List.map g_ident globs_todo) ->
+    Forall (fun x => non_void (g_typ x)) globs_todo ->
+    (forall glob, In glob globs_todo -> ~ In (g_ident glob) (map g_ident globs_done)) ->
+    init_globals globs_done g m ->
+    ℑs3 (allocate_globals globs_todo) g s m ⤳ init_globalsT (globs_todo ++ globs_done).
+Proof.
+  induction globs_todo as [| glob globs_todo IH]; intros * ND NV FRESH WF.
+  - cbn.
+    repeat rewrite ?interp3_bind, ?interp3_ret, ?bind_ret_l.
+    now apply eutt_Ret.
+  - rewrite allocate_globals_cons, interp3_bind.
+    eapply has_post_bind_strong
+      with (S := init_globalsT (glob :: globs_done)).
+    + apply allocate_global_spec.
+      * rewrite Forall_forall in NV; apply NV; left; reflexivity.
+      * apply FRESH; left; reflexivity.
+      * auto.
+    + intros [m' [ρ' [g' []]]] HInit.
+      apply has_post_weaken with (P := init_globalsT ((globs_todo ++ globs_done) ++ [glob])).
+      2: intros; now cbn; apply init_globalsT_shuffle_snoc'.
+      rewrite <- app_assoc.
+      apply IH.
+      * apply NoDup_cons_iff in ND; apply ND.
+      * inv NV; auto.
+      * intros ? IN abs.
+        rewrite map_app in abs; apply in_app_or in abs as [abs | EQ].
+        eapply FRESH; [right; eauto | auto].
+        destruct EQ as [EQ | []].
+        clear -ND EQ IN.
+        cbn in ND.
+        inv ND.
+        apply H1; rewrite EQ.
+        now apply in_map.
+      * now apply init_globals_shuffle_snoc.
+Qed.
+
+Lemma allocate_globals_spec :
+  forall (globs : list (global dtyp)) (g : global_env) (Ig : global_env -> Prop) s m,
+    (forall g, Ig g -> init_globals [] g m) ->
+    Ig g ->
+    NoDup (List.map g_ident globs) ->
+    Forall (fun x => non_void (g_typ x)) globs ->
+    ℑs3 (allocate_globals globs) g s m ⤳ init_globalsT globs.
+Proof.
+  intros.
+  pose proof app_nil_end globs as EQ.
+  rewrite EQ at 2.
+  apply allocate_globals_spec_gen; auto.
+Qed.
+
+(* TODO? Relate [init_globals] to [global_ptr_exists] *)
 
